\documentclass[12pt]{article}
%\pagestyle{empty}
\title{Equations from the parametric form of the unit circle}
\author{\null}
\date{\null}
\parindent 0px
\usepackage{amsmath,amsfonts,amssymb}
\usepackage{graphicx}
\usepackage{float}


\begin{document}
\maketitle
Consider the parametric equations for $x$ and $y$.
\\
\begin{align}
x &= \cos \theta \\
y &= \sin \theta 
\end{align}

\begin{figure}[H]
\begin{center}
	\includegraphics[scale=0.12]{desmos-graph.png}
	\caption{Unit Circle}
\end{center}
\end{figure}
Next equations (1) and (2) are differentiated
with respect to $t$.

\begin{align*}
\frac{dx}{dt} = -\sin\theta \cdot \frac{d\theta}{dt} \Longrightarrow \dot{x} = -\, \omega\cdot\sin\theta
\end{align*}
\\
\begin{align*}  
\frac{dy}{dt} = \cos\theta \cdot \frac{d\theta}{dt} \Longrightarrow \dot{y} = \omega\cdot\cos\theta
\end{align*}
\\
\\
Hence the equations for $\dot{x}$ and $\dot{y}$ are found
and also note that $\dfrac{d\theta}{dt}$ is replaced by $\omega$. \\
\begin{align}
\dot{x} &= - \, \omega \cdot \sin \theta \\
\dot{y} &= \omega \cdot \cos \theta 
\end{align}
\\ 
Equations (3) and (4) are differentiated again to obtain $\ddot{x}$ and $\ddot{y}$.

\begin{align*}
\ddot{x} &= - \, \frac{d\omega}{dt} \cdot \sin \theta - \omega^{2} \cos \theta   
\end{align*}

\begin{align*}
\ddot{y} &= \frac{d\omega}{dt} \cdot \cos \theta - \omega^{2}\sin \theta   
\end{align*}

This time $\dfrac{d^{2}\theta}{dt^{2}}$ is replaced by $\alpha$.

\begin{align}
\ddot{x} &= -\alpha \cdot \sin \theta - \omega^{2} \cdot \cos \theta \\
\ddot{y} &= \alpha \cdot \cos \theta - \omega^{2} \cdot \sin \theta
\end{align}
\\
Relationships for $\sin \theta$ and $\cos \theta$.\\[0.5cm]
From equations $(1)$, $(2)$, $(3)$ and $(4)$:
$$\sin \theta = y = -\dfrac{\dot{x}}{\omega} $$
$$\cos \theta = x =\dfrac{\dot{y}}{\omega} $$
\\
$(5)^2 + (6)^2 :$
\begin{align*}
\left(\ddot{x}\right)^{2}+\left(\ddot{y}\right)^{2} &= \left( \alpha \sin \theta + \omega^{2}\cos \theta \right)^{2} + \left( \alpha \cos \theta - \omega^{2}\sin \theta \right)^{2}\\
 													&= \alpha^{2}\sin^{2}\theta + 2\alpha \omega^{2}\sin \theta \cos \theta + \omega^{4} \cos^{2} \theta \\
 													&  \hspace{0.3 in} + \alpha^{2} \cos^{2} \theta - 2 \alpha \omega^{2} \sin \theta \cos \theta + \omega^{4}\sin^{2}\theta\\
 													&= \alpha^2 + \omega^4\\
\end{align*}

\begin{align}
\therefore \left(\ddot{x}\right)^{2}+\left(\ddot{y}\right)^{2} &= \alpha^2 + \omega^4
\end{align}
\\
Substituting $\cos\theta$ and $\sin\theta$ in equation $(5)$ terms of $x$.
$$\ddot{x} = -\alpha \left(- \frac{\dot{x}}{\omega} \right) - \omega^{2} \left( x \right)\\$$

\begin{align}
\ddot{x} = \frac{\alpha}{\omega}\dot{x} - \omega^{2} x
\end{align}
\\
Substituting $\cos\theta$ and $\sin\theta$ in equation $(6)$ terms of $y$.
$$\ddot{y} = \left(\frac{\alpha}{\omega}\right)\dot{y} - \omega^{2}(y)$$

\begin{align}
\ddot{y} = \frac{\alpha}{\omega}\dot{y}-\omega^{2}y
\end{align}



\end{document}